Concur.v: checkpoint random stuff

src/Concur.v
@@ -9,25 +9,25 @@ Require Import Omega.
 
 Set Implicit Arguments.
 
-Definition filename := nat.
-Definition filedata := nat.
+Definition filenameT := nat.
+Definition filedataT := nat.
 
-Inductive prog :=
-| Write (file : filename) (data : filedata) (rx : prog)
+Inductive progT :=
+| Write (file : filenameT) (data : filedataT) (rx : progT)
 | Exit.
 
 Inductive proc_state :=
 | NeverRan
-| Running (p : prog)
+| Running (p : progT)
 | Exited.
 
-Definition f_state := filename -> filedata.
-Definition pid := nat.
-Definition p_state := pid -> proc_state.
-Definition sys_state := (f_state * p_state)%type.
+Definition file_map := filenameT -> filedataT.
+Definition pidT := nat.
+Definition proc_map := pidT -> proc_state.
+Definition sys_state := (file_map * proc_map)%type.
 
 Definition upd {V : Type} (m : nat -> V) (a : nat) (v : V) :=
-  fun a' => if eq_nat_dec a a' then v else m a.
+  fun a' => if eq_nat_dec a a' then v else m a'.
 
 Lemma upd_eq : forall V m a (v : V),
   upd m a v a = v.
@@ -36,26 +36,40 @@ Proof.
   destruct (eq_nat_dec a a); congruence.
 Qed.
 
-Inductive exec : sys_state -> sys_state -> Prop :=
-| ExecWrite :
-  forall pid file data rx fs ps,
-  ps pid = Running (Write file data rx) ->
-  exec (fs, ps) (upd fs file data, upd ps pid (Running rx))
-| ExecExit :
-  forall pid fs ps,
-  ps pid = Running Exit ->
-  exec (fs, ps) (fs, upd ps pid Exited).
+Lemma upd_ne : forall V m a (v : V) a',
+  a <> a' ->
+  upd m a v a' = m a'.
+Proof.
+  unfold upd; intros.
+  destruct (eq_nat_dec a a'); congruence.
+Qed.
 
-Inductive execstar : sys_state -> sys_state -> Prop :=
-| ExecStarRefl :
-  forall s, execstar s s
-| ExecStarStep :
+Inductive step_pid : file_map -> proc_state -> file_map -> proc_state -> Prop :=
+| StepWrite :
+  forall file data rx fs ps,
+  ps = Running (Write file data rx) ->
+  step_pid fs ps (upd fs file data) (Running rx)
+| StepExit :
+  forall fs ps,
+  ps = Running Exit ->
+  step_pid fs ps fs Exited.
+
+Inductive step : sys_state -> sys_state -> Prop :=
+| StepChoosePid :
+  forall pid fmap fmap' pmap ps',
+  step_pid fmap (pmap pid) fmap' ps' ->
+  step (fmap, pmap) (fmap', upd pmap pid ps').
+
+Inductive star : sys_state -> sys_state -> Prop :=
+| StarRefl :
+  forall s, star s s
+| StarStep :
   forall s0 s1 s2,
-  exec s0 s1 ->
-  execstar s1 s2 ->
-  execstar s0 s2.
+  step s0 s1 ->
+  star s1 s2 ->
+  star s0 s2.
 
-Definition write_to_file (f : filename) (d : filedata) :=
+Definition write_to_file (f : filenameT) (d : filedataT) :=
   Write f d Exit.
 
 Lemma apply_eq : forall A B (f : A -> B) (x y : A),
@@ -64,18 +78,60 @@ Proof.
   congruence.
 Qed.
 
-Inductive will_not_write_to_file : filename -> prog -> Prop :=
+Inductive will_not_write_to_file : filenameT -> progT -> Prop :=
 | WNWTF_exit : forall f, will_not_write_to_file f Exit
 | WNWTF_write : forall f f' data rx, f <> f' ->
   will_not_write_to_file f rx ->
   will_not_write_to_file f (Write f' data rx).
 
-Theorem write_to_file_works_easy : forall fs ps fs' ps' newpid fn data,
-  (forall pid, exists p, ps pid = Running p -> will_not_write_to_file fn p) ->
-  ps newpid = NeverRan ->
-  execstar (fs, upd ps newpid (Running (write_to_file fn data))) (fs', ps') ->
-  ps' newpid = Exited ->
-  fs' fn = data.
+Definition wnwtf_except (pid : pidT) (fn : filenameT) (pmap : proc_map) :=
+  forall pid' p, pid' <> pid -> pmap pid' = Running p -> will_not_write_to_file fn p.
+
+Lemma wnwtf_monotonic : forall pid fn fs ps fs' ps',
+  step (fs, ps) (fs', ps') ->
+  wnwtf_except pid fn ps ->
+  wnwtf_except pid fn ps'.
+Proof.
+  inversion 1.
+  destruct (eq_nat_dec pid pid0); subst; unfold wnwtf_except; intros.
+  - rewrite upd_ne in * by auto.
+    eauto.
+  - destruct (eq_nat_dec pid0 pid'); subst.
+    + rewrite upd_eq in *; subst.
+      inversion H1.
+      specialize (H0 pid' _ H2 H7).
+      inversion H0.
+      eauto.
+    + rewrite upd_ne in * by auto.
+      eauto.
+Qed.
+
+Lemma skip_other_pids : forall fmap pmap fmap' pmap' mypid fn,
+  step (fmap, pmap) (fmap', pmap') ->
+  wnwtf_except mypid fn pmap ->
+  ((fmap fn = fmap' fn /\ pmap mypid = pmap' mypid) \/
+   (exists ps ps', pmap mypid = ps /\ pmap' = upd pmap mypid ps' /\
+    step_pid fmap ps fmap' ps')).
+Proof.
+  inversion 1.
+  destruct (eq_nat_dec pid mypid); subst; intros.
+  - right; eauto.
+  - left.
+    rewrite upd_ne by eauto; intuition.
+    inversion H1; subst; eauto.
+    unfold wnwtf_except in *.
+    specialize (H0 pid _ n H2).
+    inversion H0.
+    rewrite upd_ne; eauto.
+Qed.
+
+Theorem write_to_file_works : forall fmap pmap fmap' pmap' newpid fn data,
+  pmap newpid = NeverRan ->
+  wnwtf_except newpid fn pmap ->
+  star (fmap, upd pmap newpid (Running (write_to_file fn data)))
+       (fmap', pmap') ->
+  pmap' newpid = Exited ->
+  fmap' fn = data.
 Proof.
   intros.
 Admitted.
